% the algorithm
\subsection{A Functional Nominal C-Unification Algorithm}

% general idea for my algorithm 
\begin{frame}{General Comments About the Functional Nominal C-Unification Algorithm}
\begin{itemize}
    \item We will show a \textbf{functional} nominal C-unification algorithm, that allow us to
    unify two terms $t$ and $s$.
    \item Since the algorithm is recursive and needs to keep track of the current context,
        the substitutions made so far, the remaining terms to unify and the current
        fixpoint equations, the algorithm receives as input a quadruple 
        $(\Delta, \sigma, UnPrb, FxPntEq)$.
\end{itemize}
\end{frame}

\begin{frame}{General Comments About the Functional Nominal C-Unification Algorithm}
\begin{itemize}
    \item Call to unify terms $t$ and $s$: 
    \begin{algorithmic}[1]
        \Call{unify}{$\emptyset, id, [(t, s)], \emptyset$}.
    \end{algorithmic}
    \item The algorithm returns a list (possibly empty) of solutions. Each solution
        is of the form $(\Delta, \sigma, FxPntEq)$
\end{itemize}
\end{frame}

% resume of algorithm
\begin{frame}[allowframebreaks]{Resume of Algorithm}
\begin{algorithmic}[1]
\Procedure{unify}{$\Delta,\sigma,UnPrb, FxPntEq$}
    \If{null($UnPrb$)} 
        \State \Return {list(($\Delta, \sigma, FxPntEq$))} 
    \Else 
        \State $(t, s) \cdot UnPrb' =$ $UnPrb$
        \State [Code that analyses according to the type $t$ and $s$]
    \EndIf
\EndProcedure
\end{algorithmic}
\end{frame}

% my algorithm 
\begin{frame}[allowframebreaks]{A Functional Nominal C-Unification Algorithm}
\begin{algorithmic}[1]
\Procedure{unify}{$\Delta,\sigma,UnPrb, FxPntEq$}
    \If{null($UnPrb$)} 
        \State \Return {list(($\Delta, \sigma, FxPntEq$))} 
    \Else 
    \State $(t, s) \cdot UnPrb' =$ $UnPrb$
        \If {($s == \pi \cdot X$) and ($X$ not in $t$)}
            \State $\sigma' = \{X \rightarrow t \}$
            \State $\sigma''$ = $\sigma' \cup \sigma$ 
            \State ($\Delta'$, bool1) = appSub2Ctxt($\sigma_1, \Delta$) 
            \State $UnPrb'' = (UnPrb')\sigma' +   (FxPntEq)\sigma'$
            \Statex \Statex \Statex
            \If{bool1} \Return{\Call{unify}{$\Delta', \sigma'', UnPrb', null$}} 
            \Else  \  \Return{null}
            \EndIf
        \Else 
            \If{$t == a$} 
                \If{s == a} 
                \State \Return{\Call{unify}{$\Delta, \sigma, UnPrb', FxPntEq$}} 
                \Else
                \State \Return{null}
                \EndIf
            \Statex \Statex
            \ElsIf{$t == \pi \cdot X$}
                % if 
                \If{(X not in s)}
                    \State \Comment Similar to case above where
                    \State \Comment s is a suspension
                % else if
                \ElsIf{$(s == \pi' \cdot X)$}
                    \State $FxPntEq' = FxPntEq \cup \{((\pi')^{-1} \oplus \pi) \cdot X\}$
                    \State \Return{\Call{unify}{$\Delta, \sigma, UnPrb', FxPntEq'$}}
                % else 
                \Else \ \Return{null}
                \EndIf
            % unit
            \Statex \Statex \Statex \Statex
            \ElsIf{$t == \langle \rangle$}
                \If{$s == \langle \rangle$} 
                \State \Return{\Call{unify}{$\Delta, \sigma, UnPrb', FxPntEq$}}
                \Else \ \Return{null}
                \EndIf
            % pair
            \ElsIf{$t == \langle t_1, t_2 \rangle$}
                \If{$s == \langle s_1, s_2 \rangle$} 
                    \State $UnPrb'' = [(s_1, t_1)] + [(s_2, t_2)] + UnPrb'$
                    \State \Return{\Call{unify}{$\Delta, \sigma, UnPrb'', FxPntEq$}}
                \Else \ \Return{null}
                \EndIf
            \Statex \Statex
            % abs
            \ElsIf{$t == [a]t_1$}
                \If{$s == [a]s_1$} 
                    \State $UnPrb'' = [(t_1, s_1)] + UnPrb'$
                    \State \Return{\Call{unify}{$\Delta, \sigma, UnPrb'', FxPntEq$}}
                \ElsIf{$s == [b]s_1$}        
                    \State $(\Delta', bool1) =  fresh(a, s_1)$ 
                    \State $\Delta'' = \Delta \cup \Delta'$ 
                    \State $UnPrb'' = [(t_1, \ \ (a \ b) \ s_1)] + UnPrb'$ 
                    \If{bool1}
                        \State \Return{\Call{unify}{$\Delta'', \sigma, UnPrb'', FxPntEq$}}
                    \Else \ \Return{null}
                    \EndIf
                \Else \ \Return{null}
                \EndIf
            \ElsIf{$t == f \ t_1$} \Comment f is not commutative
                \If{$s$ != $f \ s_1$} \Return{null}
                \Else 
                    \State $UnPrb'' = [(t_1, s_1)] + UnPrb'$ 
                    \State \Return{\Call{unify}{$\Delta, \sigma, UnPrb'', FxPntEq$}}
                \EndIf
            \Statex\Statex\Statex\Statex
            \Statex\Statex
            \Else \Comment $t$ is of the form $f(t_1, t_2)$
                \If{$s$ != $f(s_1, s_2)$} \Return{null}
                \Else
                    \State $UnPrb_1 = UnPrb' + [(s_1, t_1)] + [(s_2, t_2)]$
                    \State $sol_1$ = \Call{unify}{$\Delta, \sigma, UnPrb_1, FxPntEq$}
                    \State $UnPrb_2 = UnPrb' + [(s_1, t_2)] + [(s_2, t_1)]$
                    \State $sol_2$ = \Call{unify}{$\Delta, \sigma, UnPrb_2, FxPntEq$}
                    \State \Return{\Call{append}{$sol_1, sol_2$}}
                \EndIf
            \EndIf
        \EndIf
    \EndIf
\EndProcedure
\end{algorithmic}
\end{frame}
